minimal CTL formalization with property statements in CTL

Contracts/Crowdfunding2.v
@@ -1,193 +1,72 @@
 From mathcomp.ssreflect 
 Require Import ssreflect ssrbool ssrnat eqtype ssrfun seq.
-From mathcomp
-Require Import path.
 Require Import Eqdep.
 From Heaps
 Require Import pred prelude idynamic ordtype pcm finmap unionmap heap coding. 
 From Contracts
-Require Import Automata2 CTL.
-  
+Require Import Automata2 Temporal.
+
 Set Implicit Arguments.
 Unset Strict Implicit.
 Unset Printing Implicit Defensive.
-
-(* Encoding of the Crowdfunding contract from the Scilla whitepaper *)
-(* Extended with a branching-time temporal logic *)
-
-Section Crowdfunding.
-
-Record crowdState := CS {
-   owner_mb_goal : address * nat * value;
-   backers : seq (address * value);
-   funded : bool;
-}.
-
-(* Administrative setters/getters *)
-Definition get_owner cs : address := (owner_mb_goal cs).1.1.
-Definition get_goal cs : value := (owner_mb_goal cs).2.
-Definition get_max_block cs : nat := (owner_mb_goal cs).1.2.
-
-Definition set_backers cs bs : crowdState :=
-  CS (owner_mb_goal cs) bs (funded cs).
-
-Definition set_funded cs f : crowdState :=
-  CS (owner_mb_goal cs) (backers cs) f.
-
-(* Parameters *)
-Variable init_owner : address.
-Variable init_max_block : nat.
-Variable init_goal : value.
-
-(* Initial state *)
-Definition init_state := CS (init_owner, init_max_block, init_goal) [::] false.
-
-(*********************************************************)
-(********************* Transitions ***********************)
-
-(***********************************************************)
-(**         **TEMPORAL** Correctness properties           **)
-(***********************************************************)
 
 (************************************************************************
 1. Until the funded flag has been flipped, meaning that the owner got the
 funds, the contract will have enough funds to reimburse every backer.
  ************************************************************************)
 (* Important reminder: supply pred S with crowdState and not world crowdState *)
-Variable T : Type.
-Variable w : Automata2.world T.
-Locate world.
-Definition notfunded_pred : pred crowdState :=
-  fun (w : world crowdState) => funded (state (st w)) = false.
-Definition balance_sufficient_pred : pred crowdState :=
+
+Definition notfunded : pred :=
+  fun w => funded (state (st w)) = false.
+Definition balance_sufficient : pred :=
   fun s => sumn (map snd (backers (state (st s)))) <= balance (st s).
-(*
+
 Lemma temporal_balance_backed :
   forall (w : world crowdState),
-    AllBox crowd_prot (notfunded_pred --> balance_sufficient_pred) w.
+    w |= (AG (notfunded --> balance_sufficient)).
+Proof. Admitted.
 
-
-Proof.
-  intro w.
-  unfold AllBox.
-  intros p H_fst n.
-  unfold forces.
-  unfold notfunded_pred.
-  unfold balance_sufficient_pred.
-  unfold Impl.
-  unfold not. 
-  unfold forces.
-  destruct p as [path path_fact].
-  unfold path_predicate in path_fact.
-  unfold reachability in path_fact.
-  (* Study Ilya's original proof *)
-Admitted. *)
 
 (************************************************************************
 2. Until the backer claims his donation back, the contract doesn't drop
 the records of each backer's donations.
  ************************************************************************)
-                                                                        
 
-(* Definition step_world (w : world) : world :=
-  let: CState id bal s := st w in
-  let: bc := b w in
-  let: m := inFlight w in
-  let: n := seq.find (fun t => ttag t == method m) (transitions p) in
-  let: tr := nth (idle S) (transitions p) n in
-  let: (s', out) := (tfun tr) id bal s m bc in
-  let: bal' := if out is Some m' then (bal + val m) - val m' else bal in
-  mkW m (CState id bal' s') bc out. *)
-
-(* Definition step_claim_world (w : world crowdState) : world crowdState :=
-  let: CState id bal s := st w in
-  let: bc := b w in
-  let: m := inFlight w in
-  let: (s', out) := claim_fun id bal s m bc in
-  let: bal' := if out is Some m' then (bal + val m) - val m' else bal in
-  mkW m (CState id bal' s') bc out. *)
-  
-(* Definition step_claim_state pre bc m : cstate crowdState :=
-  let: CState id bal s := pre in
-  let: (s', out) := claim_fun id bal s m bc in
-  let: bal' := if out is Some m' then (bal + val m) - val m' else bal in
-  CState id bal' s'. *)
-
-(* Definition reachable_via_message_sender (cs1 cs2 : cstate crowdState) : address -> Prop := fun n => 
-  exists (bc : bstate) (m : message),
-    step_state P cs1 bc m = cs2 /\ sender m = n. *)
-
-  (* This can't be defined solely in pred because the statement is about messages *)
-  (*
-Definition claim_from_pred (n : address) : pred crowdState :=
+Definition claim_from (n : address) : pred :=
   fun w => sender (inFlight w) = n.
-Definition donated_pred (b : address) (d : value) : pred crowdState :=
+Definition donated (b : address) (d : value) : pred :=
   fun s => (filter [pred e | e.1 == b] (backers (state (st s)))) == [::(b, d)].
        
 Lemma temporal_donation_preserved (b : address) (d : value) :
   forall (w : world crowdState),
-    (donated_pred b d w) -> AllWait crowd_prot (donated_pred b d) (claim_from_pred b) w.
-
-
-Proof.
-  intros w H_donated.
-  unfold AllWait.
-  unfold AllRelease.
-  unfold ExistsUntil.
-  unfold Neg.
-  unfold satisfies.
-  intros. destruct H.
-  destruct x as [path path_fact].
-  simpl in *.
-  destruct H.
-  destruct H0 as [spot ?].
-  destruct H0.
-  unfold first in H.
-  rewrite <- H in H_donated.
-  assert (forall j, donated_pred b d (path j)).
-  { induction j.
-    - exact H_donated.
-    - unfold path_predicate in path_fact.
-    specialize (path_fact j).
-    unfold reachability in path_fact.
-    unfold step_world in *.
-    
-    unfold first in H.
-  
-
-  Print path_predicate.
-  Abort. *)
+    (donated b d w) -> w |= (A [(donated b d) W (claim_from b)]).
+Proof. Admitted.
     
 (************************************************************************
 3. The final property: if the campaign has failed, every registered backer 
 can get its donation back.
  *************************************************************************)
-(*
-Definition balance_exceeded_pred : pred crowdState := fun w => balance (st w) < (get_goal (state (st w))).
-Definition block_exceeded (bc : bstate) : pred crowdState := fun w => get_max_block (state (st w)) < block_num bc.
 
-Definition campaign_failed (b : address) (d : value) (bc : bstate) : pred crowdState := fun w => 
-    (block_exceeded bc & balance_exceeded_pred & notfunded_pred & donated_pred b d) w.
+Definition balance_exceeded : pred := fun w => balance (st w) < (get_goal (state (st w))).
+Definition block_exceeded (bc : bstate) : pred := fun w => get_max_block (state (st w)) < block_num bc.
 
+Definition campaign_failed (b : address) (d : value) (bc : bstate) : pred := fun w => 
+    (block_exceeded bc && balance_exceeded && notfunded && donated b d) w.
 
 Lemma can_claim_back (n : address) (d : value) (bc : bstate) :
   forall w : world crowdState,
-    AllWait crowd_prot (campaign_failed n d bc) (claim_from_pred n) w.
-Proof. Abort.
-*)
+    w |= A [(campaign_failed n d bc) W (claim_from n)].
+Proof. Admitted.
+
 (************************************************************************
 4. The additional property: if the campaign has succeeded, the owner can 
 get funds to kickstart the campaign.
  *************************************************************************)
-(*
-Definition owner_gets_funds_pred : pred crowdState := fun w =>
-                                                        sender (inFlight w) = get_owner (state (st w)).
+
+Definition owner_gets_funds : pred := fun w =>
+  sender (inFlight w) = get_owner (state (st w)).
                                               
 Lemma can_get_funds :
   forall w : world crowdState,
-    AllBox crowd_prot (balance_exceeded_pred --> owner_gets_funds_pred) w.
-Proof.
-
-Abort. 
-*)
-End Crowdfunding. 
+    w |= (AG (balance_exceeded --> owner_gets_funds)).
+Proof. Admitted.
