Core/Temporal.v
@@ -1,0 +1,301 @@
+From mathcomp.ssreflect
+Require Import ssreflect eqtype.
+Require Import Eqdep.
+From Contracts
+Require Import Automata2.
+Require Import Arith Bool Omega.
+
+(* Tacticals *)
+Ltac impl_e P P_implies_Q :=
+  apply P_implies_Q in P.
+Tactic Notation "spec" hyp(H) :=
+  match type of H with ?a -> _ => 
+    let H1 := fresh in (assert (H1: a); [|generalize (H H1); clear H H1; intro H]) end.
+Tactic Notation "spec" hyp(H) constr(a) :=
+  (generalize (H a); clear H; intro H). 
+
+(* No more sections and types *)
+Definition pred := world crowdState -> Prop.
+Variable prot : Protocol crowdState.
+Definition world0_here : world crowdState := world0 prot.
+
+Definition reachability : world crowdState -> world crowdState -> Prop := fun w1 w2 => step_world prot w1 = w2.
+
+(* Path definitions *)
+Definition path := nat -> world crowdState.
+Definition first (p : path) : world crowdState := p 0.
+Definition path_predicate (p : path) := forall n, reachability (p n) (p (S n)).
+(* Good path sigma-type definitions *)
+Definition gpath : Type := {p : path & path_predicate p}.
+(* Projection functions for sigma type good paths *)
+Definition gpath_proj1 : gpath -> (nat -> world crowdState) :=
+  fun gp => match gp with
+            | existT a _ => a
+            end.
+Coercion gpath_proj1 : gpath >-> Funclass. 
+Definition gpath_proj2 (gp : gpath) : (path_predicate (gpath_proj1 gp)) :=
+  match gp with
+  | existT _ b => b
+  end.    
+(* A cacophany of path constructions *)
+(* Constructing a random path *) 
+Fixpoint step_n_times (w : world crowdState) (n : nat) :=
+  match n with
+  | 0 => w
+  | S n' => step_world prot (step_n_times w n')
+  end.
+
+Definition make_path (w : world crowdState) : path := step_n_times w.
+
+Lemma rewrite_step_world_S :
+  forall (n : nat) (w : world crowdState),
+    step_n_times w (S n) = step_world prot (step_n_times w n).
+Proof. reflexivity. Qed.
+
+Lemma step_world_swap_helper :
+  forall (n : nat) (w : world crowdState),
+    step_world prot (step_n_times w n) =
+    step_n_times (step_world prot w) n.
+Proof.
+  intros n w.
+  induction n.
+  - reflexivity.
+  - rewrite rewrite_step_world_S.
+    rewrite IHn.
+    rewrite rewrite_step_world_S.
+    reflexivity.
+Qed.
+
+Lemma step_world_swap :
+  forall n : nat,
+    step_world prot (step_n_times (step_world prot world0_here) n) =
+    step_n_times (step_world prot (step_world prot world0_here)) n.
+Proof.
+  induction n.
+  - reflexivity.
+  - rewrite step_world_swap_helper.
+    reflexivity.
+Qed.
+
+Lemma step_world_ind :
+  forall n : nat,
+    step_world prot (step_n_times world0_here n) = step_n_times world0_here (S n).
+Proof.
+  induction n.
+  - simpl; reflexivity.
+  - simpl. reflexivity.
+Qed.
+
+Lemma about_p : path_predicate (make_path world0_here).
+Proof.
+  unfold path_predicate.
+  induction n.
+  - simpl. unfold reachability. reflexivity.
+  - unfold reachability in *.
+    unfold make_path in *.
+    rewrite <- IHn.
+    simpl. reflexivity.
+Qed.
+
+Lemma about_p_hole :
+  forall w : world crowdState,
+    path_predicate (make_path w).
+Proof.
+  unfold path_predicate.
+  induction n.
+  - simpl. unfold reachability. reflexivity.
+  - unfold reachability in *.
+    unfold make_path in *.
+    rewrite <- IHn.
+    simpl. reflexivity.
+Qed.
+
+Definition gp : gpath := (existT _ (make_path world0_here) about_p).
+(* Can you make a sigma type with a dependent type? *)
+Parameter generic_world : world crowdState.
+Check (about_p_hole generic_world).
+Definition gp_hole (w : world crowdState) : gpath := (existT _ (make_path w) (about_p_hole w)).
+(* The answer is yes *)
+
+(* Constructing an offset path *)
+Definition make_offset_path (p : path) : path := fun n => p (S n).
+Definition make_offset_path' (gp : gpath) : path := fun n => gpath_proj1 gp (S n).
+Lemma about_offset_path :
+  forall p : path,
+    path_predicate p ->
+    path_predicate (make_offset_path p).
+Proof.
+  intros p H_p.
+  unfold make_offset_path.
+  unfold path_predicate in *.
+  intro n. 
+  exact (H_p (S n)).
+Qed.
+Lemma about_offset_path' :
+  forall gp : gpath,
+    path_predicate (make_offset_path' gp). 
+Proof.
+  intro gp.
+  destruct gp. unfold path_predicate in p.
+  unfold make_offset_path'.
+  unfold gpath_proj1.
+  unfold path_predicate.
+  intros n.
+  exact (p (S n)).
+Qed.
+
+Definition gp_offset (p : path) (pred : path_predicate p) : gpath :=
+  (existT _ (make_offset_path p) (about_offset_path p pred)).
+Definition gp_offset' (gp : gpath) : gpath :=
+  (existT _ (make_offset_path' gp) (about_offset_path' gp)).
+
+(* Constructing a backwards offset path *)
+Definition make_backwards_offset_path (w0 : world crowdState) (p : path) : path :=
+  fun n => match n with 0 => w0 | _ => (p (n-1)) end.
+Definition make_backwards_offset_path' (w0 : world crowdState) (gp : gpath) : path :=
+  fun n => match n with 0 => w0 | _ => (gpath_proj1 gp (n-1)) end.
+Lemma about_backwards_offset_path :
+  forall (p : path) (w0 : world crowdState),
+    path_predicate p ->
+    reachability w0 (p 0) -> 
+    path_predicate (make_backwards_offset_path w0 p).
+Proof.
+  intros p w0 H_p.
+  unfold make_backwards_offset_path.
+  unfold path_predicate in *.
+  destruct n.
+  simpl. exact H.
+  simpl. replace (n-0) with n. Focus 2. rewrite Nat.sub_0_r. reflexivity. apply (H_p n).
+Qed.
+Lemma about_backwards_offset_path' :
+  forall (gp : gpath) (w0 : world crowdState),
+    reachability w0 (gpath_proj1 gp 0) -> 
+    path_predicate (make_backwards_offset_path' w0 gp). 
+Proof.
+  intros gp w0 H_0.
+  destruct gp. unfold path_predicate in p.
+  unfold make_backwards_offset_path'.
+  unfold gpath_proj1.
+  unfold path_predicate.
+  destruct n.
+  simpl. exact H_0.
+  simpl. replace (n-0) with n. Focus 2. omega. apply (p n).
+Qed.
+Definition gp_backwards_offset
+           (w0 : world crowdState) (p : path)
+           (pred : path_predicate p)
+           (r : reachability w0 (p 0)) : gpath :=
+  (existT _ (make_backwards_offset_path w0 p) (about_backwards_offset_path p w0 pred r)).
+Definition gp_backwards_offset'
+           (w0 : world crowdState) (gp : gpath)
+           (r : reachability w0 (gpath_proj1 gp 0)) : gpath :=
+  (existT _ (make_backwards_offset_path' w0 gp) (about_backwards_offset_path' gp w0 r)).    
+(* Satisfaction definition *)
+Definition satisfies (w : world crowdState) (p : pred) : Prop := p w.
+(* I'm not sure that the following metalogic entail is necessary *)
+Definition entails (p q : pred) : Prop :=
+  forall w, (satisfies w p) -> (satisfies w q).
+Definition equiv (p q : pred) : Prop := entails p q /\ entails q p.
+ 
+Axiom LEM : forall P : Prop, P \/ ~ P.
+Notation "w '|=' p" := (satisfies w p) (at level 80, no associativity).
+
+(* Temporal operator definitions *)
+Parameter Top : pred.
+Parameter Bottom : pred.
+Axiom about_top : forall w, Top w.
+Axiom about_bottom : forall w, Bottom w -> False.
+Definition Neg p : pred := fun w => (w |= p) -> False.
+Definition Conj p q : pred := fun w => (w |= p) /\ (w |= q).
+Definition Disj p q : pred := fun w => (w |= p) \/ (w |= q).
+Definition Impl p q : pred := fun w => ~ (w |= p) \/ (w |= q).
+
+(* Temporal operator definitions *)
+(* AX says 'in every next state', all gpaths beginning with w next satisfy p. *)
+Definition AllNext (p : pred) := fun w =>  
+  forall gp : path, first gp = w -> gp 1 |= p.
+(* EX says 'in some next state', all gpaths beginning with w next satisfy p. *)
+Definition ExistsNext (p : pred) := fun w =>  
+  exists gp : path, first gp = w /\ gp 1 |= p.
+(* AG says all states along all paths beginning with  w satisfy p, including w. *)
+Definition AllBox (p : pred) := fun w =>  
+  forall gp : path, first gp = w -> forall n, gp n |= p.
+(* EG says that there exists a path beginning with w along which all states satisfy p. *)
+Definition ExistsBox (p : pred) := fun w =>  
+  exists gp : path, first gp = w /\ forall n, gp n |= p.
+(* AF says all paths beginning with w contain a future state which satisfies p. *)
+Definition AllFuture (p : pred) := fun w =>  
+  forall gp : path, first gp = w -> exists n, gp n |= p.
+(* EF says that there exists a path beginning with a future state which satisfies p. *)
+Definition ExistsFuture (p : pred) := fun w =>  
+  exists gp : path, first gp = w /\  exists n, gp n |= p.
+(* AU says that all paths beginning with w satisfy p Until q. *)
+Definition AllUntil (p q : pred) := fun w =>  
+  forall gp : path, first gp = w -> exists n, gp n |= q /\ forall m, m < n -> gp m |= p.
+(* EU says that there exists a path beginning with w that satifies p Until q. *)
+Definition ExistsUntil (p q : pred) := fun w =>  
+  exists gp : path, first gp = w /\ exists n, gp n |= q /\ forall m, m < n -> gp m |= p.
+
+(* Extended temporal operator definitions *)
+Definition AllRelease (p q : pred) := fun w => 
+  Neg (ExistsUntil (Neg p) (Neg q)) w.
+Definition ExistsRelease (p q : pred) := fun w => 
+  Neg (AllUntil (Neg p) (Neg q)) w.
+Definition AllWait (p q : pred) := fun w => 
+  AllRelease q (Disj p q) w.
+Definition ExistsWait (p q : pred) := fun w =>
+  ExistsRelease q (Disj p q) w.
+
+(* Notation definitions *)
+Notation "p <=> q" := (equiv p q) (at level 35, no associativity).
+Notation "! p" := (Neg p) (at level 60, right associativity).
+Notation "p && q" := (Conj p q) (at level 40, left associativity).
+Notation "p || q" := (Disj p q).
+Notation "p --> q" := (Impl p q) (at level 35, no associativity).
+Notation "'AG' p" := (AllBox p) (at level 35, no associativity).
+Notation "'EG' p" := (ExistsBox p) (at level 35, no associativity).
+Notation "'AX' p" := (AllNext p) (at level 35, no associativity).
+Notation "'EX' p" := (ExistsNext p) (at level 35, no associativity).
+Notation "'AF' p" := (AllFuture p) (at level 35, no associativity).
+Notation "'EF' p" := (ExistsFuture p) (at level 35, no associativity). 
+Notation "'A' '[' p 'U' q ']'" := (AllUntil p q) (at level 35, no associativity).
+Notation "'E' '[' p 'U' q ']'" := (ExistsUntil p q) (at level 35, no associativity).
+Notation "'A' '[' p 'R' q ']'" := (AllRelease p q) (at level 35, no associativity).
+Notation "'E' '[' p 'R' q ']'" := (ExistsRelease p q) (at level 35, no associativity).
+Notation "'A' '[' p 'W' q ']'" := (AllWait p q) (at level 35, no associativity).
+Notation "'E' '[' p 'W' q ']'" := (ExistsWait p q) (at level 35, no associativity).
+
+Theorem ctl_1 : forall (P : pred),
+    AG P <=> (P && AX (AG P)).
+Proof.
+  intro P. unfold equiv. unfold entails. unfold satisfies. Admitted.
+Theorem ctl_2 : forall (P : pred),
+    (P && AX (AG P)) <=> AG P.
+Proof. Admitted.
+Theorem ctl_3 : forall (P : pred),
+    EG P <=> (P && EX (EG P)).
+Proof. Admitted.      
+
+Theorem ctl_4 : forall (P : pred),
+    (P && EX (EG P)) <=> EG P.
+Proof. Admitted.
+Theorem equiv_1 : forall (P : pred),
+    AX P <=> ! (EX (! P)).
+Proof. Admitted.
+Theorem equiv_2 : forall (P : pred),
+    AF P <=> ! (EG (! P)).
+Proof. Admitted.
+Theorem equiv_3 : forall (P : pred),
+    AG P <=> ! (EF (!P)).
+Proof. Admitted.
+Theorem equiv_4 : forall (P : pred),
+    AF P <=> A [Top U P]. 
+Proof. Admitted.
+Theorem equiv_5 : forall (P : pred),
+    EF P <=> E [Top U P].
+Proof. Admitted.
+Theorem equiv_6 : forall (P Q : pred),
+    A [P U Q] <=> E [!P U (!P && !Q)] && AF Q.
+Proof. Admitted.
+
+
